challenge 6 progress

Dafny/examples/Challenge6/Challenge6Code.s.dfy
@@ -63,20 +63,82 @@ module challenge6Code{
               Ins(CALL(call1,malloc(Ptr(0,0,0,1)))),
               Ins(CALL(call2,encrypt(call,4,KEY,IV_SIZE,cipherText))),
               Ins(STORE(call2,bytes_written)),
-              Ins(CALL(call3,fwrite(bytes_written,4,1,D(Ptr(0,0,0,1))))),
-              Ins(ICMP(cmp,eq,4,call3,D(Int(0,IntType(4,false)))))])
+              Ins(CALL(call3,fwrite_empty(bytes_written,4,1,D(Ptr(0,0,0,1))))),
+              Ins(ICMP(cmp,eq,4,call3,D(Int(0,IntType(4,false))))),
+              Ins(CALL(D(Void),stateOutputDump(KEY.d,IV_SIZE.d)))])
     }
 
+
+    function challenge_prob_5_code_write_encrypted_simple_side_effect():codeRe
+    {
+
+       // [temp] dummy ptrs
+        // var call := D(Ptr(0,0,0,1));
+        var call := LV("call");
+
+        var mblock := D(Ptr(0,0,0,1));
+        var call1 := LV("call1");
+        // var call2 := D(Ptr(0,0,0,1));
+        var call2 := LV("call2");//D(Int(0,IntType(1,false)));
+        var call3 := LV("call3");//D(Int(1,IntType(4,false)));
+        var INTEGRITY_SIZE := LV("INTEGRITY_SIZE");
+
+        // var call3 := D(Ptr(0,0,0,1));
+        var call4 := D(Ptr(0,0,0,1));
+        var IV_SIZE := D(Int(16,IntType(4,false)));
+        var KEY := D(Int(16,IntType(4,false)));
+        var cipherText := D(Ptr(0,0,0,1));
+        var bytes_written := D(Ptr(0,0,0,1));
+
+        var cmp := LV("cmp");//D(Int(0,IntType(1,false)));
+        var cmp5 := D(Int(0,IntType(1,false)));
+ 
+        var var_1 := D(Ptr(0,0,0,1));
+        var var_2 := D(Int(0,IntType(4,false)));
+        var var_3 := D(Ptr(0,0,0,1));
+    
+        var conv := D(Int(0,IntType(8,false)));
+
+
+    //   %bytes_written = alloca i32, align 4
+    //   call void @llvm.lifetime.start.p0i8(i64 4, i8* nonnull %0) #24
+    //   %call = tail call noalias align 16 dereferenceable_or_null(112) i8* @malloc(i64 112) #24
+    //   tail call void @llvm.memcpy.p0i8.p0i8.i64(i8* noundef nonnull align 16 dereferenceable(112) %call, i8* noundef nonnull align 8 dereferenceable(112) getelementptr inbounds (%struct.MBlock, %struct.MBlock* @mblock, i64 0, i32 0, i64 0), i64 112, i1 false)
+    //   %call1 = tail call noalias align 16 dereferenceable_or_null(120) i8* @malloc(i64 120) #24
+    //   %call2 = tail call i32 @encrypt(i8* %call, i32 112, i8* getelementptr inbounds ([32 x i8], [32 x i8]* @KEY, i64 0, i64 0), i8* getelementptr inbounds ([16 x i8], [16 x i8]* @IV, i64 0, i64 0), i8* %call1) #24
+    //   store i32 %call2, i32* %bytes_written, align 4, !tbaa !3
+    //   %1 = load %struct._IO_FILE*, %struct._IO_FILE** @wfd, align 8, !tbaa !14
+    //   %call3 = call i64 @fwrite(i8* nonnull %0, i64 4, i64 1, %struct._IO_FILE* %1)
+    //   %cmp = icmp eq i64 %call3, 0
+    //   br i1 %cmp, label %if.then, label %if.end
+    
+    //main function block
+       Block([Ins(CALL(call,malloc(Int(0,IntType(8,false))))),
+              Ins(LLVM_MEMCPY(call,mblock,1,false)),
+              Ins(CALL(call1,malloc(Ptr(0,0,0,1)))),
+              Ins(CALL(call2,encrypt_side_effects(INTEGRITY_SIZE))),
+              Ins(STORE(call2,bytes_written)),
+              Ins(CALL(call3,fwrite_empty(bytes_written,4,1,D(Ptr(0,0,0,1))))),
+              Ins(ICMP(cmp,eq,4,call3,D(Int(0,IntType(4,false))))),
+              Ins(CALL(D(Void),stateOutputDump(KEY.d,IV_SIZE.d)))])
+    }
+
+    function stateOutputDump(KEY:Data,IV_SIZE:Data):codeSeq
+    {
+        [Ins(RET(D(KEY))),
+         Ins(RET(D(IV_SIZE)))]
+    }
  
     function encrypt(plainText:operand,size:nat,KEY:operand,IV:operand,cipherText:operand):codeSeq
     {
         [CNil]
     }
 
-    function encrypt_side_effects(plainText:operand,size:nat,KEY:operand,IV:operand,cipherText:operand):codeSeq
+    function encrypt_side_effects(INTEGRITY_SIZE:operand):codeSeq
     {
 
-        [Ins(LLVM_MEMCPY(KEY,D(Ptr(0,0,0,1)),1,false))] + encrypt(plainText,size,KEY,IV,cipherText)
+        [Ins(SUB(INTEGRITY_SIZE,1,INTEGRITY_SIZE,D(Int(1,IntType(1,false)))))] + [CNil]
+        // [Ins(LLVM_MEMCPY(KEY,D(Ptr(0,0,0,1)),1,false))] + encrypt(plainText,size,KEY,IV,cipherText)
         // lvm_Codes(Ins(LLVM_MEMCPY(KEY,D(Ptr(0,0,0,1)),1,false)),
         //           encrypt(plainText,size,KEY,IV,cipherText))    
     }
@@ -112,6 +174,11 @@ module challenge6Code{
         [Ins(RET(ptr)),CNil]
     }
 
+    function fwrite_empty(ptr:operand, size:nat, cnt:nat, file:operand):codeSeq
+    {
+        [CNil]
+    }
+
 ///////////////////////////////////////
 
     predicate validInput(s:state, input:operand)
@@ -122,14 +189,17 @@ module challenge6Code{
 
 
     predicate validStartingState(s:state)
+        // requires ValidState(s)
     {
         var call := LV("call");
         var call1 := LV("call1");
         var call2 := LV("call2");
         var call3 := LV("call3");
+        var call4 := LV("call4");
         var mblock := LV("mblock");
         var bytes_written := LV("bytes_written");
         var cmp := LV("cmp");
+        var INTEGRITY_SIZE := LV("INTEGRITY_SIZE");
         && ValidOperand(s,call)
         && ValidOperand(s,call1)
         && ValidOperand(s,call2)
@@ -137,6 +207,7 @@ module challenge6Code{
         && ValidOperand(s,mblock)
         && ValidOperand(s,cmp)
         && ValidOperand(s,bytes_written)
+        && ValidOperand(s,INTEGRITY_SIZE)
         && s.lvs["call"].Ptr?
         && s.lvs["call1"].Ptr?
         && s.lvs["call2"].Int?
@@ -144,6 +215,7 @@ module challenge6Code{
         && s.lvs["mblock"].Ptr?
         && s.lvs["bytes_written"].Ptr?
         && s.lvs["cmp"].Int?
+        && s.lvs["INTEGRITY_SIZE"].Int?
         && s.lvs["call"] == (Ptr(0,0,0,1))
         && s.lvs["call1"] == (Ptr(0,0,0,1))
         && s.lvs["call2"] == (Int(0,IntType(1,false)))
@@ -151,178 +223,14 @@ module challenge6Code{
         && s.lvs["bytes_written"] == (Ptr(0,0,0,1))
         && s.lvs["call3"] == (Int(1,IntType(4,false)))
         && s.lvs["cmp"] == Int(0,IntType(1,false))
+        && s.lvs["INTEGRITY_SIZE"] == Int(4,IntType(1,false))
         && s.m.mem[0][0].mb? 
         && s.m.mem[0][0].size == 1
+        // && operandsUnique(s,[call,call1,call2,call3,mblock,bytes_written,cmp,INTEGRITY_SIZE])
         
     }
 
-    lemma unwrapVulnBehaviors(s:state, input:operand) returns (postB:behavior)
-        requires ValidState(s);
-        requires validStartingState(s);
-
-        // -- input is valid -- ie. valid 16 bit integer 
-        requires validInput(s,input);
-        
-        ensures ValidBehaviorNonTrivial(postB);
-        ensures BehaviorEvalsCode(challenge_prob_5_code_write_encrypted_simple(),postB);
-        ensures |postB| == 9;
-        ensures behaviorOutput(postB) == [Nil,Nil,Nil,Nil,Nil,Nil,Out(s.lvs["bytes_written"]),Nil,Nil];
-
-    {
-        reveal_BehaviorEvalsCode();
-        // var call := "call";
-        reveal_ValidBehavior();
-        // reveal_ValidData();
-        var call:operand := LV("call");
-        var call1:operand := LV("call1");
-
-        var mblock:operand := LV("mblock");
-        var call2 :=LV("call2");
-        var call3 := LV("call3");
-        var cmp := LV("cmp");
-
-        // assert ValidOperand(s,call2);
-        var IV_SIZE := D(Int(16,IntType(4,false)));
-        var KEY := D(Int(16,IntType(4,false)));
-        var cipherText := D(Ptr(0,0,0,1));
-        var bytes_written := D(Ptr(0,0,0,1));
-
-        var c := challenge_prob_5_code_write_encrypted_simple();
-        assert forall cs :: cs in c.block ==> !cs.CNil?;
-        assert |c.block| == 7;
-        postB := [s] + evalCodeRE(c,s);
-       
-        var step,remainder, subBehavior := unwrapBlockWitness(postB,c.block,s);
-            step,remainder,subBehavior := unwrapBlockWitness(subBehavior,remainder,last(step));
-            step,remainder,subBehavior := unwrapBlockWitness(subBehavior,remainder,last(step));
-            step,remainder,subBehavior := unwrapBlockWitness(subBehavior,remainder,last(step));
-            step,remainder,subBehavior := unwrapBlockWitness(subBehavior,remainder,last(step));
-            step,remainder,subBehavior := unwrapBlockWitness(subBehavior,remainder,last(step));
-            step,remainder,subBehavior := unwrapBlockWitness(subBehavior,remainder,last(step));
-            step,remainder,subBehavior := unwrapBlockWitness(subBehavior,remainder,last(step));
-        
-        assert postB[0] == s;
-        assert postB[1] == evalInsRe(CALL(call,malloc(Int(0,IntType(8,false)))),s);
-        assert ValidOperand(postB[1],call);
-
-        assert NextStep(postB[1],postB[2],Step.evalInsStep(LLVM_MEMCPY(call,mblock,1,false)));
-        assert StateNext(postB[1],postB[2]);
-        assert ValidState(postB[2]);
-        assert postB[2] == evalInsRe(LLVM_MEMCPY(call,mblock,1,false),postB[1]);
-// 
-        assert postB[2] == postB[3];
-        //  assert ValidData(postB[3],OperandContents(postB[3],call1));
-        // assert validEvalIns(CALL(call1,malloc(Ptr(0,0,0,1))),postB[2],postB[3]);
-        assert NextStep(postB[2],postB[3],Step.evalInsStep(CALL(call1,malloc(Ptr(0,0,0,1)))));
-        assert ValidState(postB[3]);
-
-        // assert ValidInstruction(postB[3],CALL(call2,encrypt(call,4,KEY,IV_SIZE,cipherText)));
-        // assert c.block[3] == Ins(CALL(call2,encrypt(call,4,KEY,IV_SIZE,cipherText)));
-        assert NextStep(postB[3],postB[4],Step.evalInsStep(CALL(call2,encrypt(call,4,KEY,IV_SIZE,cipherText))));
-        assert postB[3] == postB[4];
-        assert ValidState(postB[4]);
-        
-        // assert ValidInstruction(postB[4],STORE(call2,bytes_written));
-        // assert c.block[4] == Ins(STORE(call2,bytes_written));
-        // var s' := postB[4].(m := evalStore(postB[4].m,OperandContents(postB[4],bytes_written).bid,OperandContents(postB[4],bytes_written).offset,OperandContents(postB[4],call2)));
-        // assert MemValid(s'.m);
-        assert NextStep(postB[4],postB[5],Step.evalInsStep(STORE(call2,bytes_written)));
-        assert ValidState(postB[5]);
-        
-
-        assert ValidInstruction(postB[5],CALL(call3,fwrite(bytes_written,4,1,D(Ptr(0,0,0,1)))));
-        assert postB[6] == evalInsRe(CALL(call3,fwrite(bytes_written,4,1,D(Ptr(0,0,0,1)))),postB[5]);
-        var subB := unwrapFwriteWitness(postB[5],call3,bytes_written,4,1,D(Ptr(0,0,0,1)),postB[6]);
-        // var subB := evalBlockRE(fwrite(bytes_written,4,1,D(Ptr(0,0,0,1))),postB[5]);
-        // assert fwrite(bytes_written,4,1,D(Ptr(0,0,0,1))) == [Ins(RET(bytes_written)),CNil];
-        // var metaB := evalCodeRE(Ins(RET(bytes_written)),postB[5]);
-        // var s' := postB[5].(o := Out(OperandContents(postB[5],bytes_written)));
-        // assert metaB == [s'];
-        // assert ValidState(s');
-        // var theRest := evalBlockRE([CNil],s');
-        // assert theRest == [s'];
-        // assert subB == [s',s'];
-        // assert NextStep(subB[0],subB[1],Step.stutterStep());
-        assert behaviorOutput(subB) == [Out(OperandContents(postB[5],bytes_written)),Out(OperandContents(postB[5],bytes_written))];
-
-        assert ValidBehavior(subB);
-        assert ValidOperand(last(subB),call3);
-
-        // var stepS,remainderS, subBehaviorS := unwrapBlockWitness(subB,(fwrite(bytes_written,4,1,D(Ptr(0,0,0,1)))),postB[5]);
-
-        // assert subB == evalCodeRE(Ins(RET(bytes_written)),postB[5]);
-        // assert |subB| == 2;
-        // assert c.block[5] == Ins(CALL(call3,fwrite(bytes_written,4,1,D(Ptr(0,0,0,1)))));
-        assert NextStep(postB[5],postB[6],Step.evalInsStep(CALL(call3,fwrite(bytes_written,4,1,D(Ptr(0,0,0,1))))));
-        assert postB[6].ok;
-
-        assert postB[6].o == Out(OperandContents(postB[5],bytes_written));// == stateUpdateVar(last(subB),call3,OperandContents(last(subB),call3));
-        // assert postB[6].o == Out(OperandContents(postB[5],bytes_written));
-        assert StateNext(postB[5],postB[6]);
-        assert ValidState(postB[6]);
-
-        // // assert ValidInstruction(postB[6],ICMP(cmp,eq,4,call3,D(Int(0,IntType(4,false)))));
-        // // assert c.block[6] == Ins(ICMP(cmp,eq,4,call3,D(Int(0,IntType(4,false)))));
-        assert NextStep(postB[6],postB[7],Step.evalInsStep(ICMP(cmp,eq,4,call3,D(Int(0,IntType(4,false))))));
-        assert StateNext(postB[6],postB[7]);
-        assert ValidState(postB[7]);
-
-        // // LAST STEP
-        assert postB[7] == postB[8];
-        assert ValidState(postB[8]);
-        assert NextStep(postB[7],postB[8],Step.stutterStep());
-        assert StateNext(postB[7],postB[8]);
-
-        assert ValidBehaviorNonTrivial(postB);
-        assert BehaviorEvalsCode(c,postB);
-        assert |postB| == 9;
-        assert behaviorOutput(postB) == [Nil,Nil,Nil,Nil,Nil,Nil,Out(postB[5].lvs["bytes_written"]),Nil,Nil];
-        // assert NextStep(postB[5],postB[6],Step.evalInsStep(CALL(call3,fwrite(bytes_written,4,1,D(Ptr(0,0,0,1))))));
-
-
-                // assert postB[3] == evalInsRe(CALL(call1,malloc(Ptr(0,0,0,1))),s);
-
-        // assert NextStep(postB[2],postB[3],Step.evalInsStep(CALL(call1,malloc(Ptr(0,0,0,1)))));
-        // assert StateNext(postB[2],postB[3]);
-
-
-    }
-
-    lemma unwrapFwriteWitness(s:state,dst:operand,ptr:operand, size:nat, cnt:nat, file:operand,sNext:state) returns (b:behavior)
-        requires ValidState(s)
-        requires ValidOperand(s,ptr)
-        requires ValidOperand(s,dst)
-        requires sNext == evalInsRe(CALL(dst,fwrite(ptr,size,cnt,file)),s)
-        requires ValidInstruction(s,CALL(dst,fwrite(ptr,size,cnt,file)));
-        // ensures 
-        ensures |b| > 0
-        ensures ValidBehavior(b);
-        ensures ValidOperand(last(b),dst);
-        ensures behaviorOutput(b) == [Out(OperandContents(s,ptr)),Out(OperandContents(s,ptr))];
-        ensures b == evalBlockRE(fwrite(ptr,size,cnt,file),s);
-        ensures NextStep(s,sNext,Step.evalInsStep(CALL(dst,fwrite(ptr,size,cnt,file))));
-        ensures StateNext(s,sNext);
-
-
-    {
-        // assert ValidInstruction(s,CALL(dst,fwrite(ptr,size,cnt,file)));
-        var subB := evalBlockRE(fwrite(ptr,size,cnt,file),s);
-        assert fwrite(ptr,size,cnt,file) == [Ins(RET(ptr)),CNil];
-        var metaB := evalCodeRE(Ins(RET(ptr)),s);
-        assert ValidInstruction(s,RET(ptr));
-        assert metaB == [evalInsRe(RET(ptr),s)];
-        var s' := s.(o := Out(OperandContents(s,ptr)));
-        assert metaB == [s'];
-        assert ValidState(s');
-        var theRest := evalBlockRE([CNil],s');
-        assert theRest == [s'];
-        assert subB == [s',s'];
-        assert NextStep(subB[0],subB[1],Step.stutterStep());
-        // assert validEvalIns(ins,s,s');
-        assert sNext.ok ==> NextStep(s,sNext,Step.evalInsStep(CALL(dst,fwrite(ptr,size,cnt,file))));
-        return subB;
-    }
-
+   
 }
 // **** MAIN.C MAIN WHILE LOOP ****
 
