Dafny/examples/Challenge6/Challenge6CodeLemmasSideEffect.i.dfy
@@ -1,0 +1,583 @@
+include "../../LLVM/llvmREFACTOR.i.dfy"
+include "../../LLVM/types.dfy"
+include "../../LLVM/control_flow.i.dfy"
+include "../../LLVM/behaviorLemmas.i.dfy"
+include "../../Libraries/Seqs.s.dfy"
+include "../../LLVM/memory.i.dfy"
+include "Challenge6Code.s.dfy"
+include "../../LLVM/Operations/binaryOperations.i.dfy"
+
+module challenge6CodeLemmasSideEffect{
+    import opened control_flow
+    import opened LLVM_defRE
+    import opened types
+    import opened Collections__Seqs_s
+    import opened behavior_lemmas
+    import opened memory
+    import opened challenge6Code
+    import opened binary_operations_i
+
+// -- hechenxi@umich : chenxi
+
+lemma unwrapVulnBehaviors(s:state, input:operand, c:codeRe) returns (preB:behavior)
+        requires ValidState(s);
+        requires validStartingState(s);
+        requires c == challenge_prob_5_code_write_encrypted_simple_side_effect();
+
+        // -- input is valid -- ie. valid 16 bit integer 
+        requires validInput(s,input);
+        
+        // ensures ValidBehaviorNonTrivial(preB);
+        ensures BehaviorEvalsCode(challenge_prob_5_code_write_encrypted_simple_side_effect(),preB);
+        ensures |preB| == 10;
+        ensures preB[0] == s;
+        
+        // ensures StateNext(preB[0],preB[1]);
+        // ensures StateNext(preB[1],preB[2]);
+        // ensures ValidState(preB[0]);
+        // ensures ValidState(preB[1]);
+        // ensures ValidState(preB[2]);
+        // ensures preB[2] == preB[3];
+        // ensures ValidState(preB[3]);
+        // ensures preB[3] == preB[4];
+        // ensures ValidState(preB[4]);
+        // ensures ValidState(preB[5]);
+        // ensures StateNext(preB[0],preB[1]);
+        // ensures StateNext(preB[1],preB[2]);
+        // ensures StateNext(preB[2],preB[3]);
+        // ensures StateNext(preB[3],preB[4]);
+        // ensures StateNext(preB[4],preB[5]);
+        // ensures StateNext(preB[5],preB[6]);
+        // ensures ValidState(preB[6]);
+        // ensures StateNext(preB[6],preB[7]);
+        // ensures ValidState(preB[7]);
+        // ensures StateNext(preB[7],preB[8]);
+        // ensures ValidState(preB[8]);
+        // ensures StateNext(preB[8],preB[9]);
+        // ensures ValidState(preB[9]);
+        // // ensures preB == [s] + evalCodeRE(c,s);
+        // // ensures 
+        // ensures behaviorOutput(preB) == [Nil,
+        //                                 Nil,
+        //                                 Nil,
+        //                                 Nil,
+        //                                 Nil,
+        //                                 Nil,
+        //                                 Nil,
+        //                                 Nil,
+        //                                 SubOut([Out(Int(16,IntType(4,false))),Out(Int(16,IntType(4,false))),Out(Int(16,IntType(4,false)))]),
+        //                                 SubOut([Out(Int(16,IntType(4,false))),Out(Int(16,IntType(4,false))),Out(Int(16,IntType(4,false)))])];
+
+
+
+    {
+        reveal_BehaviorEvalsCode();
+        // reveal_ValidBehavior();
+
+        var call:operand := LV("call");
+        var call1:operand := LV("call1");
+        var mblock:operand := LV("mblock");
+        var call2 :=LV("call2");
+        var call3 := LV("call3");
+        assert OperandContents(s,call3).itype.size == 4;
+        var INTEGRITY_SIZE := LV("INTEGRITY_SIZE");
+
+        var cmp := LV("cmp");
+        var IV_SIZE := D(Int(16,IntType(4,false)));
+        var KEY := D(Int(16,IntType(4,false)));
+        var cipherText := D(Ptr(0,0,0,1));
+        var bytes_written := D(Ptr(0,0,0,1));
+
+        // var c := challenge_prob_5_code_write_encrypted_simple();
+        assert |c.block| == 8;
+        preB := [s] + evalCodeRE(c,s);
+       
+        var step,remainder,subBehavior := unwrapBlockWitness(preB,c.block,s);
+
+            step,remainder,subBehavior := unwrapBlockWitness(subBehavior,remainder,last(step));
+            step,remainder,subBehavior := unwrapBlockWitness(subBehavior,remainder,last(step));
+            step,remainder,subBehavior := unwrapBlockWitness(subBehavior,remainder,last(step));
+            step,remainder,subBehavior := unwrapBlockWitness(subBehavior,remainder,last(step));
+            step,remainder,subBehavior := unwrapBlockWitness(subBehavior,remainder,last(step));
+            step,remainder,subBehavior := unwrapBlockWitness(subBehavior,remainder,last(step));
+            step,remainder,subBehavior := unwrapBlockWitness(subBehavior,remainder,last(step));
+            step,remainder,subBehavior := unwrapBlockWitness(subBehavior,remainder,last(step));
+
+        assert preB[0] == s;
+        assert preB[1] == evalInsRe(CALL(call,malloc(Int(0,IntType(8,false)))),s);
+        assert ValidOperand(preB[1],call);
+
+        assert NextStep(preB[1],preB[2],Step.evalInsStep(LLVM_MEMCPY(call,mblock,1,false)));
+        assert StateNext(preB[1],preB[2]);
+        assert ValidState(preB[2]);
+        assert preB[2] == evalInsRe(LLVM_MEMCPY(call,mblock,1,false),preB[1]);
+// 
+        assert preB[2] == preB[3];
+        assert NextStep(preB[2],preB[3],Step.evalInsStep(CALL(call1,malloc(Ptr(0,0,0,1)))));
+        assert ValidState(preB[3]);
+
+        assert preB[4] == evalInsRe(CALL(call2,encrypt_side_effects(INTEGRITY_SIZE)),preB[3]);
+        assert ValidInstruction(preB[3],CALL(call2,encrypt_side_effects(INTEGRITY_SIZE)));
+        var sha := unwrapEncryptSideEffectsWitness(preB[3],call2,INTEGRITY_SIZE,preB[4]);
+        assert ValidState(preB[4]);
+        assert ValidBehavior(sha);
+        assert ValidOperand(last(sha),call2);
+        assert NextStep(preB[3],preB[4],Step.evalInsStep(CALL(call2,encrypt_side_effects(INTEGRITY_SIZE))));
+        // var stemp := stateUpdateVar(last(sha),call2,OperandContents(last(sha),call2));
+        assert validEvalIns(CALL(call2,encrypt_side_effects(INTEGRITY_SIZE)),preB[3],preB[4]);
+        assert call2.LV?;
+        assert  StateNext(preB[3],preB[4]);
+        assert OperandContents(preB[3],INTEGRITY_SIZE).val == 4;
+        assert ValidOperand(preB[4],INTEGRITY_SIZE);
+        assert OperandContents(preB[4],INTEGRITY_SIZE).val == 3;
+
+        // assert preB[4] == last(sha).(o := Nil);
+                // assert OperandContents(preB[4],INTEGRITY_SIZE).val == 3;
+
+        // assert preB[3] == preB[4];
+        assert ValidState(preB[4]);
+         assert preB[5] == evalInsRe(STORE(call2,bytes_written),preB[4]);
+         assert ValidOperand(preB[4],call2);// && 
+         assert ValidOperand(preB[4],bytes_written);
+        //  assert ValidInstruction(preB[4],STORE(call2,bytes_written));
+        // assert NextStep(preB[4],preB[5],Step.evalInsStep(STORE(call2,bytes_written)));
+        // assert ValidState(preB[5]);
+        
+
+        // assert ValidInstruction(preB[5],CALL(call3,fwrite(bytes_written,4,1,D(Ptr(0,0,0,1)))));
+        // assert preB[6] == evalInsRe(CALL(call3,fwrite_empty(bytes_written,4,1,D(Ptr(0,0,0,1)))),preB[5]);
+        // assert preB[5] == preB[6];
+        // assert ValidState(preB[6]);
+
+        // assert StateNext(preB[5],preB[6]);
+        // assert ValidState(preB[6]);
+        
+        // assert cmp.LV?;
+        // // var r := D(Int(0,IntType(4,false)));
+        // // assert  IntFits(r.d.val,r.d.itype);
+        // var src2 := validZero16bitInt(preB[6]);
+        // assert ValidOperand(preB[6],call3);// 
+        // assert ValidOperand(preB[6],src2);
+        // assert && isInt(OperandContents(preB[6],call3));// 
+        // assert && isInt(OperandContents(preB[6],src2));
+        // assert OperandContents(preB[6],call3).itype.size == 4;
+        // assert !OperandContents(preB[6],call3).itype.signed;
+        // intsTypeMatch(OperandContents(preB[6],call3),OperandContents(preB[6],src2));
+        // assert typesMatch(OperandContents(preB[6],call3),OperandContents(preB[6],src2));
+
+        // // assert (Int(1,IntType(4,false))) == OperandContents(preB[6],call3);
+        // assert ValidInstruction(preB[6],ICMP(cmp,eq,4,call3,src2));
+
+        // assert preB[7] == evalInsRe(ICMP(cmp,eq,4,call3,src2),preB[6]);
+        // // var s' := stateUpdateVar(preB[6],cmp,evalICMP(eq,4,OperandContents(preB[6],call3),OperandContents(preB[6],src2)));
+
+
+        // assert NextStep(preB[6],preB[7],Step.evalInsStep(ICMP(cmp,eq,4,call3,src2)));
+        // assert StateNext(preB[6],preB[7]);
+        // assert ValidState(preB[7]);
+
+        // assert ValidInstruction(preB[7],CALL(D(Void),stateOutputDump(KEY.d,IV_SIZE.d)));
+        // // assert c[7] == CALL(D(Void),stateOutputDump(KEY,IV_SIZE));
+        // assert preB[8] == evalInsRe(CALL(D(Void),stateOutputDump(KEY.d,IV_SIZE.d)),preB[7]);
+        // var dump := unwrapDumpWitness(preB[7],KEY.d,IV_SIZE.d,preB[8]);
+        // assert NextStep(preB[7],preB[8],Step.evalInsStep(CALL(D(Void),stateOutputDump(KEY.d,IV_SIZE.d))));   
+        // assert preB[8].o == SubOut([Out((Int(16,IntType(4,false)))),Out(Int(16,IntType(4,false))),Out(Int(16,IntType(4,false)))]);
+
+        // // // // LAST STEP
+        // assert preB[8] == preB[9];
+        // equalStatesAreStutter(preB[8],preB[9]);
+        // // assert ValidState(preB[8]);
+        // // assert NextStep(preB[7],preB[8],Step.stutterStep());
+        // assert StateNext(preB[8],preB[9]);
+
+        // // // assert ValidBehaviorNonTrivial(preB);
+        // // // assert BehaviorEvalsCode(c,preB);
+        // assert |preB| == 10;
+        // assert behaviorOutput(preB) == [Nil,
+        //                                 Nil,
+        //                                 Nil,
+        //                                 Nil,
+        //                                 Nil,
+        //                                 Nil,
+        //                                 Nil,
+        //                                 Nil,
+        //                                 SubOut([Out(Int(16,IntType(4,false))),Out(Int(16,IntType(4,false))),Out(Int(16,IntType(4,false)))]),
+        //                                 SubOut([Out(Int(16,IntType(4,false))),Out(Int(16,IntType(4,false))),Out(Int(16,IntType(4,false)))])];
+
+
+    }
+
+
+
+//  lemma vulnBehaviorIsValid(s:state, input:operand) returns (preB:behavior)
+//         requires ValidState(s);
+//         requires validStartingState(s);
+
+//         // -- input is valid -- ie. valid 16 bit integer 
+//         requires validInput(s,input);
+
+//     {
+//         reveal_ValidBehavior();
+//         reveal_BehaviorEvalsCode();
+//         var c := challenge_prob_5_code_write_encrypted_simple_side_effect();
+//         var x := unwrapVulnBehaviors(s,input,c);
+//         assert ValidBehaviorNonTrivial(x);
+//         assert BehaviorEvalsCode(c,x);
+
+//         // assert behaviorOutput(x) == [Nil,Nil,Nil,Nil,Nil,Nil,Out(x[5].lvs["bytes_written"]),Nil,Nil];
+
+//         // assert BehaviorEvalsCode(c,preB);
+//     }
+
+
+    lemma equalStatesAreStutter(s:state,s':state)
+        requires s==s'
+        requires ValidState(s);
+        ensures ValidState(s');
+        ensures NextStep(s,s',Step.stutterStep());
+        ensures StateNext(s,s');
+    {
+         assert ValidState(s');
+         assert NextStep(s,s',Step.stutterStep());
+         assert StateNext(s,s');
+    }
+
+    lemma intsTypeMatch(x:Data,y:Data)
+        requires (isInt(x) && isInt(y))
+        requires x.itype.size == y.itype.size
+        requires x.itype.signed == y.itype.signed
+        ensures typesMatch(x,y);
+    {
+        assert typesMatch(x,y);
+    }
+
+    function validZero16bitInt(s:state) : (val:operand)
+        ensures val.D?;
+        ensures val.d.Int?;
+        ensures ValidData(s, val.d)
+        ensures !val.d.itype.signed
+        ensures val.d.itype.size == 4
+    {
+        var val := D(Int(0,IntType(4,false)));
+        assert  IntFits(val.d.val,val.d.itype);
+        val
+    }
+
+    lemma unwrapEncryptSideEffectsWitness(s:state,dst:operand,INTEGRITY_SIZE:operand, sNext:state) returns (b:behavior)
+        requires ValidState(s)
+        requires ValidOperand(s,INTEGRITY_SIZE)
+        requires ValidOperand(s,dst)
+        requires dst != INTEGRITY_SIZE;
+        requires dst.LV?;
+        requires dst.l in s.lvs;
+        requires INTEGRITY_SIZE.LV?;
+        requires INTEGRITY_SIZE.l in s.lvs;
+        requires isInt(OperandContents(s,INTEGRITY_SIZE));
+        requires OperandContents(s,INTEGRITY_SIZE).itype.size == 1;
+        requires typesMatch(OperandContents(s,INTEGRITY_SIZE),OperandContents(s,D(Int(1,IntType(1,false)))))
+        requires OperandContents(s,INTEGRITY_SIZE).val == 4;
+        requires sNext == evalInsRe(CALL(dst,encrypt_side_effects(INTEGRITY_SIZE)),s);
+        requires ValidInstruction(s,CALL(dst,encrypt_side_effects(INTEGRITY_SIZE)));
+        requires s.o == Nil
+        ensures ValidBehavior(b);
+        ensures |b| == 3
+        ensures ValidOperand(last(b),dst)
+        ensures ValidOperand(last(b),INTEGRITY_SIZE) && OperandContents(last(b),INTEGRITY_SIZE).Int?
+        ensures OperandContents(last(b),INTEGRITY_SIZE).val == 3;
+         ensures NextStep(s,sNext,Step.evalInsStep(CALL(dst,encrypt_side_effects(INTEGRITY_SIZE))));
+        ensures StateNext(s,sNext);
+        ensures ValidState(sNext);
+        ensures ValidOperand(sNext,INTEGRITY_SIZE);
+        // ensures OperandContents(s,dst) == OperandContents(last(b),dst);
+        ensures sNext == last(b).(o := Nil);
+        ensures behaviorOutput(b) == [Nil,Nil,Nil]
+    {
+        reveal_behaviorOutput();
+        reveal_ValidBehavior();
+        var subB := [s] + evalCodeRE(Block(encrypt_side_effects(INTEGRITY_SIZE)),s);
+        assert encrypt_side_effects(INTEGRITY_SIZE) == [Ins(SUB(INTEGRITY_SIZE,1,INTEGRITY_SIZE,D(Int(1,IntType(1,false))))),CNil];
+        var step,remainder,subBehavior := unwrapBlockWitness(subB,encrypt_side_effects(INTEGRITY_SIZE),s);
+        step,remainder,subBehavior := unwrapBlockWitness(subBehavior,remainder,last(step));
+        // step,remainder,subBehavior := unwrapBlockWitness(subBehavior,remainder,last(step));
+         assert subB[0] == s;
+         assert subB[1] == evalInsRe(SUB(INTEGRITY_SIZE,1,INTEGRITY_SIZE,D(Int(1,IntType(1,false)))),s);
+         assert NextStep(subB[0],subB[1],Step.evalInsStep(SUB(INTEGRITY_SIZE,1,INTEGRITY_SIZE,D(Int(1,IntType(1,false))))));
+         assert subB[1] == subB[2];
+        assert subB[2] == stateUpdateVar(s,INTEGRITY_SIZE,evalSUB(1,OperandContents(s,INTEGRITY_SIZE),(Int(1,IntType(1,false)))));
+        assert dst.l in subB[1].lvs;
+        assert dst.l != INTEGRITY_SIZE.l;
+        assert forall lv :: (lv in s.lvs && lv != INTEGRITY_SIZE.l) ==> subB[1].lvs[lv] == s.lvs[lv];
+
+        assert s.lvs[dst.l] == subB[1].lvs[dst.l];
+        //  assert OperandContents(s,dst) == OperandContents(subB[1],dst);
+         equalStatesAreStutter(subB[1],subB[2]);
+         assert StateNext(subB[1],subB[2]);
+         assert |subB| == 3;
+         assert subB[2] == last(subB);
+         assert  OperandContents(subB[2],INTEGRITY_SIZE).val == 3;
+         assert ValidBehavior(subB);
+         return subB;
+    }
+
+    lemma unwrapDumpWitness(s:state,op1:Data,op2:Data,sNext:state) returns (b:behavior)
+        requires ValidState(s)
+        requires ValidData(s,op1)
+        requires ValidData(s,op2)
+        requires sNext == evalInsRe(CALL(D(Void),stateOutputDump(op1,op2)),s)
+        requires ValidInstruction(s,CALL(D(Void),stateOutputDump(op1,op2)));
+        requires s.o == Nil
+
+        ensures |b| == 4
+        ensures ValidBehavior(b);
+        ensures ValidOperand(last(b),D(Void));
+        // ensures ValidOperand(b[1],op2);
+        ensures behaviorOutput(b) == [Nil,Out(op1),Out(op2),Out(op2)];
+        ensures NextStep(s,sNext,Step.evalInsStep(CALL(D(Void),stateOutputDump(op1,op2))));
+        ensures StateNext(s,sNext);
+        ensures ValidState(sNext);
+        ensures sNext.o == SubOut([Out(op1),Out(op2),Out(op2)]);
+
+    {
+        reveal_behaviorOutput();
+        var subB := [s] + evalCodeRE(Block(stateOutputDump(op1,op2)),s);// alBlockRE(stateOutputDump(op1,op2),s);
+        assert stateOutputDump(op1,op2) == [Ins(RET(D(op1))),Ins(RET(D(op2)))];
+
+        var step,remainder,subBehavior := unwrapBlockWitness(subB,stateOutputDump(op1,op2),s);
+        step,remainder,subBehavior := unwrapBlockWitness(subBehavior,remainder,last(step));
+        step,remainder,subBehavior := unwrapBlockWitness(subBehavior,remainder,last(step));
+        
+        assert subB[0] == s;
+        assert NextStep(subB[0],subB[1],Step.evalInsStep(RET(D(op1))));
+        assert ValidState(subB[1]);
+        assert subB[1].o == Out(op1);
+        assert NextStep(subB[1],subB[2],Step.evalInsStep(RET(D(op2))));
+        assert ValidState(subB[2]);
+        assert subB[2].o == Out(op2);
+        assert subB[2] == subB[3];
+        equalStatesAreStutter(subB[2],subB[3]);
+        assert StateNext(subB[2],subB[3]);
+        assert behaviorOutput(subB) == [Nil,Out(op1),Out(op2),Out(op2)];
+        assert sNext == evalInsRe(CALL(D(Void),stateOutputDump(op1,op2)),s);
+        assert sNext.ok;
+        var rest := evalBlockRE(stateOutputDump(op1,op2),s);
+        assert subB == [s] + rest;
+        assert behaviorOutput(rest) == [Out(op1),Out(op2),Out(op2)];
+        assert sNext.o == SubOut(behaviorOutput(rest));
+        return subB;
+    }
+
+
+
+    lemma unwrapFwriteWitness(s:state,dst:operand,ptr:operand, size:nat, cnt:nat, file:operand,sNext:state) returns (b:behavior)
+        requires ValidState(s)
+        requires ValidOperand(s,ptr)
+        requires ValidOperand(s,dst)
+        requires isInt(OperandContents(s,dst));
+        requires sNext == evalInsRe(CALL(dst,fwrite(ptr,size,cnt,file)),s)
+        requires ValidInstruction(s,CALL(dst,fwrite(ptr,size,cnt,file)));
+        // ensures 
+        ensures |b| > 0
+        ensures ValidBehavior(b);
+        ensures ValidOperand(last(b),dst);
+        ensures behaviorOutput(b) == [Out(OperandContents(s,ptr)),Out(OperandContents(s,ptr))];
+        ensures b == evalBlockRE(fwrite(ptr,size,cnt,file),s);
+        ensures NextStep(s,sNext,Step.evalInsStep(CALL(dst,fwrite(ptr,size,cnt,file))));
+        ensures StateNext(s,sNext);
+        ensures ValidState(sNext);
+        ensures isInt(OperandContents(sNext,dst));
+        ensures OperandContents(sNext,dst).itype.size == OperandContents(s,dst).itype.size;
+        ensures OperandContents(sNext,dst).itype.signed == OperandContents(s,dst).itype.signed;
+
+
+    {
+        // assert ValidInstruction(s,CALL(dst,fwrite(ptr,size,cnt,file)));
+        var subB := evalBlockRE(fwrite(ptr,size,cnt,file),s);
+        assert fwrite(ptr,size,cnt,file) == [Ins(RET(ptr)),CNil];
+        var metaB := evalCodeRE(Ins(RET(ptr)),s);
+        assert ValidInstruction(s,RET(ptr));
+        assert metaB == [evalInsRe(RET(ptr),s)];
+        var s' := s.(o := Out(OperandContents(s,ptr)));
+        assert metaB == [s'];
+        assert ValidState(s');
+        var theRest := evalBlockRE([CNil],s');
+        assert theRest == [s'];
+        assert subB == [s',s'];
+        assert NextStep(subB[0],subB[1],Step.stutterStep());
+        // assert validEvalIns(ins,s,s');
+        assert sNext.ok ==> NextStep(s,sNext,Step.evalInsStep(CALL(dst,fwrite(ptr,size,cnt,file))));
+        return subB;
+    }
+
+
+}
+
+//  lemma unwrapVulnBehaviors(s:state, input:operand, c:codeRe) returns (preB:behavior)
+//         requires ValidState(s);
+//         requires validStartingState(s);
+//         requires c == challenge_prob_5_code_write_encrypted_simple();
+
+//         // -- input is valid -- ie. valid 16 bit integer 
+//         requires validInput(s,input);
+        
+//         // ensures ValidBehaviorNonTrivial(preB);
+//         ensures BehaviorEvalsCode(challenge_prob_5_code_write_encrypted_simple(),preB);
+//         ensures |preB| == 9;
+//         ensures preB[0] == s;
+//                 ensures StateNext(preB[0],preB[1]);
+
+//         ensures StateNext(preB[1],preB[2]);
+//                 ensures ValidState(preB[0]);
+//         ensures ValidState(preB[1]);
+
+//         ensures ValidState(preB[2]);
+//         ensures preB[2] == preB[3];
+//         ensures ValidState(preB[3]);
+//         ensures preB[3] == preB[4];
+//         ensures ValidState(preB[4]);
+//         ensures ValidState(preB[5]);
+//         ensures StateNext(preB[0],preB[1]);
+
+//         ensures StateNext(preB[1],preB[2]);
+
+//         ensures StateNext(preB[2],preB[3]);
+
+//         ensures StateNext(preB[3],preB[4]);
+//         ensures StateNext(preB[4],preB[5]);
+
+//         ensures StateNext(preB[5],preB[6]);
+//         ensures ValidState(preB[6]);
+//         ensures StateNext(preB[6],preB[7]);
+//         ensures ValidState(preB[7]);
+//         ensures StateNext(preB[7],preB[8]);
+//         ensures ValidState(preB[8]);
+//         ensures preB == [s] + evalCodeRE(c,s);
+//         // ensures 
+//         ensures behaviorOutput(preB) == [Nil,Nil,Nil,Nil,Nil,Nil,Out(Ptr(0,0,0,1)),Nil,Nil];
+
+
+//     {
+//         reveal_BehaviorEvalsCode();
+//         // reveal_ValidBehavior();
+
+//         var call:operand := LV("call");
+//         var call1:operand := LV("call1");
+//         var mblock:operand := LV("mblock");
+//         var call2 :=LV("call2");
+//         var call3 := LV("call3");
+//                 assert OperandContents(s,call3).itype.size == 4;
+
+//         var cmp := LV("cmp");
+//         var IV_SIZE := D(Int(16,IntType(4,false)));
+//         var KEY := D(Int(16,IntType(4,false)));
+//         var cipherText := D(Ptr(0,0,0,1));
+//         var bytes_written := D(Ptr(0,0,0,1));
+
+//         // var c := challenge_prob_5_code_write_encrypted_simple();
+//         assert |c.block| == 7;
+//         preB := [s] + evalCodeRE(c,s);
+       
+//         var step,remainder,subBehavior := unwrapBlockWitness(preB,c.block,s);
+
+//             step,remainder,subBehavior := unwrapBlockWitness(subBehavior,remainder,last(step));
+//             step,remainder,subBehavior := unwrapBlockWitness(subBehavior,remainder,last(step));
+//             step,remainder,subBehavior := unwrapBlockWitness(subBehavior,remainder,last(step));
+//             step,remainder,subBehavior := unwrapBlockWitness(subBehavior,remainder,last(step));
+//             step,remainder,subBehavior := unwrapBlockWitness(subBehavior,remainder,last(step));
+//             step,remainder,subBehavior := unwrapBlockWitness(subBehavior,remainder,last(step));
+//             step,remainder,subBehavior := unwrapBlockWitness(subBehavior,remainder,last(step));
+        
+//         assert preB[0] == s;
+//         assert preB[1] == evalInsRe(CALL(call,malloc(Int(0,IntType(8,false)))),s);
+//         assert ValidOperand(preB[1],call);
+
+//         assert NextStep(preB[1],preB[2],Step.evalInsStep(LLVM_MEMCPY(call,mblock,1,false)));
+//         assert StateNext(preB[1],preB[2]);
+//         assert ValidState(preB[2]);
+//         assert preB[2] == evalInsRe(LLVM_MEMCPY(call,mblock,1,false),preB[1]);
+// // 
+//         assert preB[2] == preB[3];
+//         assert NextStep(preB[2],preB[3],Step.evalInsStep(CALL(call1,malloc(Ptr(0,0,0,1)))));
+//         assert ValidState(preB[3]);
+
+//         assert NextStep(preB[3],preB[4],Step.evalInsStep(CALL(call2,encrypt(call,4,KEY,IV_SIZE,cipherText))));
+//         assert preB[3] == preB[4];
+//         assert ValidState(preB[4]);
+        
+//         assert NextStep(preB[4],preB[5],Step.evalInsStep(STORE(call2,bytes_written)));
+//         assert ValidState(preB[5]);
+        
+
+//         assert ValidInstruction(preB[5],CALL(call3,fwrite(bytes_written,4,1,D(Ptr(0,0,0,1)))));
+//         assert preB[6] == evalInsRe(CALL(call3,fwrite(bytes_written,4,1,D(Ptr(0,0,0,1)))),preB[5]);
+//         var subB := unwrapFwriteWitness(preB[5],call3,bytes_written,4,1,D(Ptr(0,0,0,1)),preB[6]);
+
+//         assert behaviorOutput(subB) == [Out(OperandContents(preB[5],bytes_written)),Out(OperandContents(preB[5],bytes_written))];
+//         assert OperandContents(preB[5],bytes_written) == Ptr(0,0,0,1);
+//         assert ValidBehavior(subB);
+//         assert ValidOperand(last(subB),call3);
+
+//         assert NextStep(preB[5],preB[6],Step.evalInsStep(CALL(call3,fwrite(bytes_written,4,1,D(Ptr(0,0,0,1))))));
+//         // assert preB[6].ok;
+
+//         // assert preB[6].o == Out(OperandContents(preB[5],bytes_written));// == stateUpdateVar(last(subB),call3,OperandContents(last(subB),call3));
+//         assert StateNext(preB[5],preB[6]);
+//         assert ValidState(preB[6]);
+        
+//         assert cmp.LV?;
+//         // var r := D(Int(0,IntType(4,false)));
+//         // assert  IntFits(r.d.val,r.d.itype);
+//         var src2 := validZero16bitInt(preB[6]);
+//         assert ValidOperand(preB[6],call3);// 
+//         assert ValidOperand(preB[6],src2);
+//         assert && isInt(OperandContents(preB[6],call3));// 
+//         assert && isInt(OperandContents(preB[6],src2));
+//         assert OperandContents(preB[6],call3).itype.size == 4;
+//         assert !OperandContents(preB[6],call3).itype.signed;
+//         intsTypeMatch(OperandContents(preB[6],call3),OperandContents(preB[6],src2));
+//         assert typesMatch(OperandContents(preB[6],call3),OperandContents(preB[6],src2));
+
+//         // assert (Int(1,IntType(4,false))) == OperandContents(preB[6],call3);
+//         assert ValidInstruction(preB[6],ICMP(cmp,eq,4,call3,src2));
+
+//         assert preB[7] == evalInsRe(ICMP(cmp,eq,4,call3,src2),preB[6]);
+//         // var s' := stateUpdateVar(preB[6],cmp,evalICMP(eq,4,OperandContents(preB[6],call3),OperandContents(preB[6],src2)));
+
+
+//         assert NextStep(preB[6],preB[7],Step.evalInsStep(ICMP(cmp,eq,4,call3,src2)));
+//         assert StateNext(preB[6],preB[7]);
+//         assert ValidState(preB[7]);
+
+//         // // // // LAST STEP
+//         assert preB[7] == preB[8];
+//         equalStatesAreStutter(preB[7],preB[8]);
+//         // assert ValidState(preB[8]);
+//         // assert NextStep(preB[7],preB[8],Step.stutterStep());
+//         assert StateNext(preB[7],preB[8]);
+
+//         // assert ValidBehaviorNonTrivial(preB);
+//         // assert BehaviorEvalsCode(c,preB);
+//         assert |preB| == 9;
+//         assert behaviorOutput(preB) == [Nil,Nil,Nil,Nil,Nil,Nil,Out(preB[5].lvs["bytes_written"]),Nil,Nil];
+
+
+//     }
+
+    // lemma test(s:state, input:operand) returns (preB:behavior)
+    //     requires ValidState(s);
+    //     requires validStartingState(s);
+
+    //     // -- input is valid -- ie. valid 16 bit integer 
+    //     requires validInput(s,input);
+
+    // {
+    //     reveal_ValidBehavior();
+    //     reveal_BehaviorEvalsCode();
+    //     var c := challenge_prob_5_code_write_encrypted_simple();
+    //     var x := unwrapVulnBehaviors(s,input,c);
+    //     assert ValidBehaviorNonTrivial(x);
+    //     assert BehaviorEvalsCode(c,x);
+
+    //     // assert behaviorOutput(x) == [Nil,Nil,Nil,Nil,Nil,Nil,Out(x[5].lvs["bytes_written"]),Nil,Nil];
+
+    //     // assert BehaviorEvalsCode(c,preB);
+    // }
